Complete search example
Using a modified loop invariant made it much simpler. Moved the previous version together with multiple little exercise-lemmas
to a separate file.

progs/verif_search.v
@@ -3,19 +3,17 @@ Require Import VST.floyd.proofauto.
 Require Import VST.progs.search.
 Instance CompSpecs : compspecs. make_compspecs prog. Defined.
 Definition Vprog : varspecs. mk_varspecs prog. Defined.
-
 From mathcomp.ssreflect Require Import ssreflect.
 
 Definition Znth_opt { X : Type } (n : Z) (lst : list X) : option X :=
   Znth n (map Some lst) None.
 
 Section SearchSpec.
-
   Variable X : Type.
 
   (* Search for an element within a list.
    *
-   * Return
+   * Return:
    * - The 0-based index of the first match on success,
    * - None otherwise.
    *)
@@ -28,139 +26,18 @@ Section SearchSpec.
       Znth_opt i lst = Some target /\
       forall (j : Z), 0 <= j < i -> Znth_opt j lst <> Some target ).
 
-  Lemma search_ind :
-    search_spec0 -> forall (target : X) (lst : list X) (i : Z),
-      0 <= i < Zlength lst ->
-      search target (sublist 0 i lst) = None ->
-      Znth_opt i lst <> Some target ->
-      search target (sublist 0 (i + 1) lst) = None.
+  Lemma search_none :
+    search_spec0 -> forall (target : X) (lst : list X),
+      ( ( forall (i : Z), 0 <= i < Zlength lst -> Znth_opt i lst <> Some target )
+        -> search target lst = None ).
   Proof.
-    move => H_spec target lst i H_i H_search H_nth.
-    destruct (search _ (sublist 0 (i+1) lst)) as [ j | ] eqn:H_eq; first exfalso; last done.
-    (* Assume on the contrary that search result is positive *)
+    move => H_spec target lst H_asm.
+    destruct (search target lst) as [ i | _ ] eqn:H_eq; last done.
+    (* Need to discharge `search target lst = Some i` *)
     move : H_eq.
-    move /H_spec => [] H_j [] H_jth H_minimal.
-    rewrite Zlength_sublist in H_j; [ | omega | omega ].
-    have : (j < i \/ j = i).
-      (* Need to exclude j > i *)
-      move : (Ztrichotomy j i) => [ | [] ]; [ tauto | tauto | move => H_j_gt_i ].
-      omega.
-    move => [ H_j_lt_i | H_i_j ].
-    * (* j < i *)
-      (* If we can find some j < i such that the search is successful,
-         we can also find a smallest one. *)
-      suffices H_contr: (search target (sublist 0 i lst) = Some j).
-        move : H_search.
-        rewrite H_contr.
-        discriminate.
-        apply H_spec; repeat split; try omega.
-        * rewrite Zlength_sublist; omega.
-        * rewrite /Znth_opt -sublist_map Znth_sublist; try omega.
-          rewrite /Znth_opt -sublist_map Znth_sublist in H_jth; try omega.
-          assumption.
-        * move => j0 H_j0.
-          move/(_ j0 H_j0) in H_minimal.
-          rewrite /Znth_opt -sublist_map Znth_sublist; try omega.
-          rewrite /Znth_opt -sublist_map Znth_sublist in H_minimal; try omega.
-          assumption.
-    * (* j = i *)
-      rewrite H_i_j /Znth_opt -sublist_map Znth_sublist in H_jth; [ | omega | omega ].
-      replace (i + 0) with i in H_jth by omega.
-      contradiction.
-  Qed.
-
-  Lemma search_nil :
-    search_spec0 -> forall (target : X), search target [] = None.
-  Proof.
-    rewrite/search_spec0 => H_spec target.
-    move/(_ target []) in H_spec.
-    destruct (search target []) as [ i | ] eqn:H_search; last reflexivity.
-    (* Assume search has found something *)
-    move/(_ i) in H_spec.
+    move /H_spec => [] H_i [] H_match.
     exfalso.
-    have : @Znth_opt X i [] = Some target by tauto.
-    rewrite/Znth_opt //= Znth_nil. discriminate.
-  Qed.
-
-  (* That must be somewhere in the std library... *)
-  Definition is_some { X : Type } : option X -> bool :=
-    option_rect (fun _ => bool) (fun _ => true) false.
-
-  Definition search_spec1 : Prop :=
-    forall (target : X) (lst : list X) (i : Z),
-    search target lst = Some i <-> (
-      0 <= i < Zlength lst          /\
-      Znth_opt i lst = Some target /\
-      ~ In target (sublist 0 i lst)).
-
-  Lemma In_Znth { A : Type} (lst : list A) (x d : A) :
-    In x lst -> ( exists (i : Z), 0 <= i < Zlength lst /\ Znth i lst d = x ).
-  Proof.
-    move /(In_nth _ _ d) => [] iN [] ? ?.
-    exists (Z.of_nat iN).
-    split; first split.
-     * by apply Nat2Z.is_nonneg.
-    * rewrite Zlength_correct; omega.
-    * rewrite /Znth.
-      have H_i0 : (Z.of_nat iN) >= 0 by omega.
-      rewrite zlt_false; last by assumption.
-      by rewrite Nat2Z.id.
-  Qed.
-
-  Proposition search_spec_equiv01 :
-    search_spec0 <-> search_spec1.
-  Proof.
-    have H_lem : forall (i : Z) (lst : list X) (target : X), 0 <= i < Zlength lst ->
-      ~ In target (sublist 0 i lst)
-      <-> ( forall (j : Z), 0 <= j < i -> Znth_opt j lst <> Some target ).
-    {
-      move => i lst target H_i.
-      split; [ move => H_in | move => H_nth ].
-      + move => j H_j_lt_i H_nth.
-        apply H_in.
-        have H_nth' : (Znth j lst target) = target
-          by move : H_nth; rewrite /Znth_opt (Znth_map target);
-             [ case | omega ].
-        have <- : (Znth j (sublist 0 i lst) target) = target
-          by rewrite -{2}H_nth' Znth_sublist; first f_equal; omega.
-        apply Znth_In; split; last rewrite Zlength_sublist; omega.
-      + move /(In_Znth _ _ target) => [].
-        move => j [] H_j H_jth.
-        move /(_ j) in H_nth.
-        rewrite Zlength_sublist in H_j; [ | omega | omega ].
-        apply H_nth; first omega.
-        rewrite Znth_sublist in H_jth; [ | omega | omega ].
-        replace (j + 0) with j in H_jth by omega.
-        rewrite /Znth_opt (Znth_map target); [ by f_equal | omega ].
-    }
-    (* After this lemma, it's just a matter of writing out
-     * and splitting all definitions, in both directions *)
-    split;
-      move => H_asm target lst i;
-      move /(_ i lst target) in H_lem;
-      move /(_ target lst i) in H_asm;
-      tauto.
-  Qed.
-
-  Definition search_spec2 : Prop :=
-    forall (target : X) (lst : list X) (i : Z),
-    search target lst = Some i <-> (
-      0 <= i < Zlength lst          /\
-      Znth_opt i lst = Some target /\
-      search target (sublist 0 i lst) = None ).
-
-  Proposition search_spec_equiv12 :
-    search_spec1 <-> search_spec2.
-  Admitted.
-
-  Proposition search_spec_equiv02 :
-    search_spec0 <-> search_spec2.
-  Proof.
-    (* Make prover more aware of the previous equivalences
-       by putting them in the proof context. *)
-    pose search_spec_equiv01.
-    pose search_spec_equiv12.
-    tauto.
+    apply (H_asm i); assumption.
   Qed.
 
 End SearchSpec.
@@ -174,62 +51,12 @@ Module ZTy <: Ty.
 End ZTy.
 
 Module Type SearchImplementation ( XTy : Ty ).
-
   Export XTy.
-
   Parameter search : X -> list X -> option Z.
   Parameter search_spec : search_spec0 X search.
-
 End SearchImplementation.
 
-
-Module SearchSpecImpliesDecidableEquality (XTy : Ty) (SImp : SearchImplementation XTy).
-
-  Import SImp.
-
-  Definition eqX (x y : X) : bool :=
-    match search x [y] with
-    | Some _ => true
-    | None   => false
-    end.
-
-  Lemma search_refl: forall (x : X), search x [x] = Some 0.
-  Proof.
-    move => x.
-    apply search_spec; split; [ | split ].
-    + by rewrite Zlength_cons //=.
-    + by rewrite /Znth_opt /Znth //=.
-    + move => j [] ? ?; exfalso; omega.
-  Qed.
-
-  Lemma eqX_spec : forall (x y : X), eqX x y = true <-> x = y.
-  Proof.
-    split.
-    + (* Assume x, y are equal wrt. eqX / search *)
-      rewrite/eqX.
-      set search_res := search x [y].
-      (* Search must have been successful *)
-      destruct search_res as [ i | ] eqn:H_search; [ move => _ | discriminate ].
-      (* Apply spec *)
-      move /search_spec in H_search.
-      move : H_search => [] H_len [] H_nth H_no_earlier.
-      (* Only possible search index is i=0 because [y] has length 1 *)
-      have H_i0 : i = 0.
-      -  move: H_len => [] H_0_le_i H_i_lt_len.
-         rewrite Zlength_cons //= in H_i_lt_len.
-           omega.
-      rewrite H_i0 /Znth_opt /Znth //= in H_nth.
-        by inversion H_nth.
-    + (* Assume x and y are Leibniz equal *)
-      move => ->.
-      by rewrite /eqX search_refl.
-  Qed.
-
-End SearchSpecImpliesDecidableEquality.
-
-
 Module C_search_verify (Imp : SearchImplementation ZTy).
-
   Import Imp.
 
   Definition Csearch_spec : ident * funspec :=
@@ -267,21 +94,16 @@ Module C_search_verify (Imp : SearchImplementation ZTy).
 
   Definition Gprog := ltac:(with_library prog [Csearch_spec]).
 
-  Locate "PROP".
-  Print mpred. Print sublist. Locate "=". Search eqb.
-
   Lemma body_search_alt: semax_body Vprog Gprog f_search_alt Csearch_spec.
   Proof.
     pose search_spec.
     (* Our second alternative for the search spec fits best *)
-    have search_spec2 : search_spec2 X search
-      by apply search_spec_equiv02; assumption.
     start_function.
     forward.
     forward_while
       (EX i:Z,
-         PROP  (0 <= i <= length;
-                search target (sublist 0 i contents) = None)
+            PROP  (0 <= i <= length;
+                   forall (j : Z), 0 <= j < i -> Znth_opt j contents <> Some target )
          LOCAL ( temp _i (Vint (Int.repr i ) );
                  temp _length (Vint ( Int.repr length ) );
                  temp _target (Vint (Int.repr target));
@@ -292,9 +114,8 @@ Module C_search_verify (Imp : SearchImplementation ZTy).
     * (* Loop invariant holds initially; take i = 0 *)
       Exists 0.
       entailer!.
-      (* Initially, sublist is empty, and hence search result is None;
-         That was proved from the spec as `search_nil` above. *)
-      by rewrite sublist_nil (search_nil X search search_spec).
+      (* Condition 0 <= j < j is unsatisfiable *)
+      move => ? ?; exfalso; omega.
     * (* Some type checking *)
       entailer!.
     * (* Loop invariant is indeed an invariant *)
@@ -327,13 +148,13 @@ Module C_search_verify (Imp : SearchImplementation ZTy).
           apply Forall_Znth; [ by split | by assumption ].
         have H_rep_target : repable_signed target by assumption.
         move /(_ H_rep_cont_i H_rep_target) in H5.
-        (* Now we know that there's also a match of abstrac integers
+        (* Now we know that there's also a match of abstract integers
            and can use this together with the loop-assumption to show
            that our return value matches the value of the abstract
            search function. *)
         have -> : (search target contents = Some i).
         {
-          apply search_spec2.
+          apply search_spec.
           by rewrite /Znth_opt (Znth_map 0); repeat split; try f_equal.
         }
         entailer.
@@ -355,165 +176,32 @@ Module C_search_verify (Imp : SearchImplementation ZTy).
       forward.
       Exists (i+1).
       entailer!.
-      by apply search_ind.
+      (* Need to prove loop invariant for i+1, so essentially we have to split
+         the assumption 0 <= j < i+1 into the cases 0 <= j < i and j = i, using
+         the loop assumption and the outcome of the branch, respectively. *)
+      move => j H_j_le.
+      have : j < i \/ j = i.
+      {
+        (* Only need to discharge j > i *)
+        move : (Ztrichotomy j i) => [ | []];
+           [ tauto | tauto | move => H_j_gt_i; exfalso; omega ].
+      }
+      move => [ H_j_lt_i | -> ].
+      + (* j < i *)
+        by apply H3; omega.
+      + (* j = i *)
+        assumption.
     * (* We've left the loop - check function postcondition *)
       assert_PROP (Zlength contents = length). {
         entailer!. do 2 rewrite Zlength_map. reflexivity.
       }
-      move : H3.
-      have -> : i = length by omega.
-      rewrite sublist_same; [ | done | done ] => H_search_res.
+      have H_i_len : i = length by omega.
+      rewrite H_i_len.
+      rewrite H_i_len in H3.
       forward.
-      rewrite H_search_res.
+      have -> : search target contents = None
+        by apply search_none.
       entailer.
-Qed.
-
-
-(* The canonical implementation of a search function for integers *)
-Module LinearSearch : SearchImplementation ZTy.
-
-  Import ZTy.
-
-  Fixpoint search (target: X) (lst: list X) { struct lst } : option Z :=
-    match lst with
-    | nil => None
-    | cons a lst' =>
-      if Z.eqb a target then
-        Some 0%Z
-      else
-        option_map (Z.add 1) (search target lst')
-    end.
-
-  (** Helper lemmas *)
-
-  Lemma sublist_empty { X : Type } (a b : Z) :
-    @sublist X a b [] = [].
-  Proof.
-    by rewrite /sublist skipn_nil firstn_nil.
   Qed.
 
-  Lemma Znth_opt_some { X : Type } (n : Z) (d : X) (lst : list X) :
-    0 <= n < Zlength lst -> Znth_opt n lst = Some (Znth n lst d).
-  Proof.
-    move => H_len.
-    by rewrite /Znth_opt (Znth_map d).
-  Qed.
-
-  Lemma sublist_0_pos { X : Type } (i : Z) (x : X) (lst : list X) :
-    0 < i <= Zlength( x :: lst )
-    -> sublist 0 i (x :: lst) = x :: ( sublist 0 (i - 1) lst ).
-  Proof.
-    move => [].
-    move => H_1_le_i H_i_len.
-    replace (x :: lst) with ([x] ++ lst) by trivial.
-    rewrite Zlength_cons in H_i_len.
-    rewrite sublist0_app2; [ done | rewrite Zlength_cons //=; omega ].
-  Qed.
-
-  Lemma option_map_inj { X Y : Type } (f : X -> Y) (x : option X) :
-    option_map f x = None -> x = None.
-  Proof. by case: x. Qed.
-
-  Lemma search_none_cons0 (lst : list Z) (target : Z) (x : Z) :
-    search target (x :: lst) = None ->  Z.eqb x target = false.
-  Proof.
-    move => H.
-    apply not_true_is_false => R.
-      by rewrite /search R in H.
-  Qed.
-
-  Lemma search_none_cons1 (lst : list Z) (target : Z) (x : Z) :
-    search target (x :: lst) = None ->
-    search target lst = None.
-  Proof.
-    move => H. move : (H). move: H => /search_none_cons0.
-    rewrite {1}/search => ->.
-      by move /option_map_inj.
-  Qed.
-
-  Lemma Znth_opt_cons { X : Type } (lst : list X) (x : X) (i : Z):
-    0 < i -> Znth_opt i (x :: lst) = Znth_opt (i - 1) lst.
-  Admitted.
-
-  Lemma search_result (lst : list Z) (target : Z) (i : Z) :
-    0 <= i < Zlength lst
-    -> search target (sublist 0 i lst) = None  (* No match up to ith entry *)
-    -> Znth_opt i lst = Some target            (* i-th entry matches       *)
-    -> search target lst = Some i.             (* Then search result is i  *)
-  Proof.
-    (* Induction lst, the empty case being contradictory *)
-    elim: lst i => [ | a lst IH] i; first by move => [] ? /Zlt_not_le.
-    move /(_ (i-1)) in IH.
-    (* Distinguish i=0 and i<>0 *)
-    move => [] H0 H1.
-    move: (Zle_lt_or_eq 0 i H0) => [ H_0lti | <- ].
-    * (* 0 < i *)
-      rewrite sublist_0_pos.
-      move => H_search.
-      Focus 2.
-      split.
-    + by assumption.
-    + by omega.
-      rewrite Znth_opt_cons;
-        last by assumption.
-      move => H_Znth.
-      rewrite /search (search_none_cons0 (sublist 0 (i-1) lst) _ a) -/search;
-        last by assumption.
-      rewrite -/search IH //=.
-    + apply f_equal; omega.
-    + rewrite Zlength_cons in H1; omega.
-    + by apply (search_none_cons1 _ _ a).
-      * (* 0 = i *)
-        rewrite /Znth_opt /Znth //=.
-        move => _. case => ->;
-                    by rewrite Z.eqb_refl.
-  Qed.
-
-  Lemma search_spec :
-    forall (target : X) (lst : list X) (i : Z),
-    search target lst = Some i <-> (
-      0 <= i < Zlength lst          /\
-      Znth_opt i lst = Some target /\
-      forall (j : Z), 0 <= j < i -> Znth_opt j lst <> Some target ).
-  Proof.
-  Admitted.
-
-  Eval compute in search 5 [ 1; 4; 2; 63; 5; 12 ].
-  Eval compute in search 7 [ 1; 4; 2; 63; 5; 12 ].
-
-End LinearSearch.
-
-
-  (* Definition search_spec : ident * funspec := *)
-  (*   DECLARE _search *)
-  (*     WITH arr: val, sh: share, contents: list Z, length: Z, target: Z *)
-  (*     PRE [ _arr OF (tptr tint), _length OF tint, _target OF tint ] *)
-  (*       PROP (readable_share sh; *)
-  (*             (* Make sure abstract integers are within *) *)
-  (* (*                the representable range of machine integers *) *)
-  (*             0 <= length <= Int.max_signed; *)
-  (*             Forall (fun x => Int.min_signed <= x <= Int.max_signed ) contents) *)
-  (*       LOCAL ( temp _arr    arr; *)
-  (*               temp _length (Vint (Int.repr length)); *)
-  (*               temp _target (Vint (Int.repr target)) ) *)
-  (*       SEP   ( (* length represents the contents of the *) *)
-  (* (*                  length `length` array starting at `array`. *) *)
-  (*               data_at sh (tarray tint length) *)
-  (*                          (map Vint (map Int.repr contents)) *)
-  (*                          arr ) *)
-  (*     POST [ tint ] *)
-  (*       PROP  (True) *)
-  (*       LOCAL ( temp ret_temp ( *)
-  (*                      (* Convert list index to pointer *) *)
-  (*                      match (search target contents) with *)
-  (*                      | None (* Nothing found, expect NULL pointe *) *)
-  (*                          => nullval *)
-  (*                      | Some idx%Z (* Add index to array base *) *)
-  (*                          => field_address0 (tarray tint length) *)
-  (*                                           [ArraySubsc idx] *)
-  (*                                           arr *)
-  (*                      end ) ) *)
-  (*       SEP   ( (* Data hasn't been modified or freed *) *)
-  (*               data_at sh (tarray tint length) *)
-  (*                          (map Vint (map Int.repr contents)) *)
-  (*                          arr ). *)
+End C_search_verify.
